TODO.md
@@ -1,7 +1,7 @@
 __Auto Issues:__
-* Getting unsat core from zipperposition.
 * HOL to FOL. Do this in the verified checker. Introduce new etoms to represent instancecs of higher-order functions.
 * When we matched against ``Eq`` in monomorphization, we found that some type arguments of other constants got unified with ``Prop``, which created a bunch of junk lemma. Find out whether something similar happened in Duper.
+* Matcher issue: Please use ``Lean.Meta.Match.getEquationsFor``. Maybe ``getMatcherInfo?`` is also useful.
 * Implement native interpretation
 * Improve portfolio mode script. Download E and zipperposition from the web.
 * Floating point numbers
@@ -21,7 +21,6 @@ __Auto Issues:__
 * Report errors when monomorphization fails.
 * Better inhabitation reasoning (a new lambaseterm ctor "nonempty"). Support divide and conquer for inhabitation reasoning in verified checker?
 * Create an interface that invokes the verified checker for duper.
-* Eta-expand (=) (??) (!!) when sending problem to zipperposition.
 * Premise Selection:
   * https://lean-forward.github.io/pubs/geesing_msc_thesis.pdf
   * https://github.com/aalistairr/ps-lean
@@ -30,9 +29,6 @@ __Auto Issues:__
 * Benchmarks:
   * GRUNGE: https://arxiv.org/abs/1903.02539
   * Seventeen benchmark: https://matryoshka-project.github.io/pubs/seventeen.pdf
-* Justification:
-  * Duper is fine on problems suitable for hammers
-  * Duper can do something that metis can't
 
 __Lean Issues:__
 * ``cases`` fails on some simple examples. E.g, ``cases h : a.beq b`` fails if the goal contains term
